cpp2v: Structured names under `--ast2`
Command-line:

- Add `--ast2` to print structured names for templated code
- Add `--trace=choices` to print a debug trace
- Add `--name-test` to test structured names

Also,

- Add `loc::loc`, `ClangPrinter::{error_prefix,debug_dump}` for diagnostics
- Generalize `print.list` to work with `llvm::ArrayRef<T>`
- Adjust `print.list` to pass only the list element to its callback
- Fix `VisitAutoType`. In dependent contexts, the deduced type for
`auto` can be (a `QualType` carrying) nullptr.
- Pass location information into `ClangPrinter::printQualType`
(usually) and several other functions that might receive `nullptr`
- (In progress) Avoid `assert(b && "message")` when checking clang's
"invariants" since we no longer enable assertions

include/Location.hpp
@@ -1,0 +1,223 @@
+/*
+ * Copyright (c) 2024 BedRock Systems, Inc.
+ * This software is distributed under the terms of the BedRock Open-Source License.
+ * See the LICENSE-BedRock file in the repository root for details.
+ */
+#pragma once
+#include <optional>
+#include <clang/Basic/SourceLocation.h>
+
+namespace llvm {
+class raw_ostream;
+class StringRef;
+}
+
+namespace clang {
+class ASTContext;
+class Decl;
+class DeclContext;
+class FunctionDecl;
+class NamedDecl;
+class QualType;
+class Stmt;
+class Type;
+class TypeLoc;
+class TypeSourceInfo;
+class TemplateArgumentLoc;
+class CXXRecordDecl;
+class CXXBaseSpecifier;
+}
+
+// Low-level utilities shared by the structured name printer and
+// locations. (In general, these cannot safely use locations.)
+namespace structured {
+using namespace llvm;
+using namespace clang;
+
+// TODO: Drop this in favor of printing `?null`
+void locfree_warn(const Decl&, const ASTContext&, StringRef);
+
+const FunctionDecl* recoverFunction(const Decl& decl);
+
+/// A variant of NamedDecl::getNameForDiagnostic that adds template
+/// parameters, function parameters, and function qualifiers.
+raw_ostream& printNameForDiagnostics(raw_ostream&, const NamedDecl&,
+                                     const ASTContext&);
+} // namespace structured
+
+namespace loc {
+
+using namespace llvm;
+using namespace clang;
+
+/*
+Roughly, a sum of a few types that can be dumped
+and have an optional location.
+*/
+class Loc final {
+private:
+    // Used to impose invariants
+    template<typename T>
+    struct box {
+        const T* unbox;
+        const T* operator->() const { return unbox; }
+        const T& operator*() const { return *unbox; }
+    };
+
+    enum class Kind {
+        Decl,
+        Stmt,
+        TypeLoc,
+        QualType,
+        Type,
+        Tsi,
+        Tal,
+    } kind;
+
+    union {
+        const Decl* decl;
+        const Stmt* stmt;
+        const box<TypeLoc> typeloc;	// type is non-null
+        const box<TypeSourceInfo> tsi;	// type is non-null
+        const box<QualType> qualtype;	// type is non-null
+        const Type* type;
+        const TemplateArgumentLoc* tal;
+    } u;
+
+    Loc(const box<TypeLoc>& t) : kind{Kind::TypeLoc}, u{.typeloc = t} {}
+    Loc(const box<TypeSourceInfo>& t) : kind{Kind::Tsi}, u{.tsi = t} {}
+    Loc(const box<QualType>& t) : kind{Kind::QualType}, u{.qualtype = t} {}
+public:
+    Loc() = delete;
+    Loc(const Decl& d) : kind{Kind::Decl}, u{.decl = &d} {}
+    Loc(const Stmt& s) : kind{Kind::Stmt}, u{.stmt = &s} {}
+    Loc(const Type& t) : kind{Kind::Type}, u{.type = &t} {}
+    Loc(const TemplateArgumentLoc& a) : kind{Kind::Tal}, u{.tal = &a} {}
+
+    static std::optional<Loc> mk(const TypeLoc&);
+    static std::optional<Loc> mk(const TypeSourceInfo&);
+    static std::optional<Loc> mk(const QualType&);
+
+    // Location (may be invalid)
+
+    SourceLocation getLoc() const;
+
+    // Short description
+
+    raw_ostream& describe(raw_ostream&, const ASTContext&) const;
+
+    // Clang's AST dump
+
+    raw_ostream& dump(raw_ostream&, const ASTContext&) const;
+};
+
+using loc = std::optional<Loc>;
+
+// Introduction
+
+inline constexpr loc none = std::nullopt;
+
+// Use constructors when they can't go wrong
+template<typename T> loc of(T& ref) { return {Loc{ref}}; }
+
+// Use factory methods to check side-conditions
+template<> inline loc of<>(const TypeLoc& ref) { return Loc::mk(ref); }
+template<> inline loc of<>(TypeLoc& ref) { return Loc::mk(ref); }
+template<> inline loc of<>(const TypeSourceInfo& ref) { return Loc::mk(ref); }
+template<> inline loc of<>(TypeSourceInfo& ref) { return Loc::mk(ref); }
+template<> inline loc of<>(const QualType& ref) { return Loc::mk(ref); }
+template<> inline loc of<>(QualType& ref) { return Loc::mk(ref); }
+
+// Avoid an ambiguous constructor
+template<> loc of<>(const DeclContext&);
+template<> loc of<>(DeclContext&);
+
+// Handle pointers
+template<typename T>
+loc
+of(T* ptr) {
+    return ptr ? of(*ptr) : none;
+}
+
+/// `loc::of(t)` if that's defined and has a location; otherwise,
+/// `fallback`
+template<typename T>
+loc
+refine(loc fallback, T t) {
+    auto loc = of(t);
+    return loc && loc->getLoc().isValid() ? loc : fallback;
+}
+
+// Formatting
+
+// Describe loc (e.g., "Var x"), if present.
+inline bool
+can_describe(loc loc) {
+    return loc.has_value();
+}
+struct Describe {
+    loc location;
+    const ASTContext& context;
+};
+inline Describe
+describe(loc loc, const ASTContext& context) {
+    return {loc, context};
+}
+raw_ostream& operator<<(raw_ostream&, Describe);
+
+// Dump loc (presumed under decl) or decl, if either is present.
+struct Dump {
+    loc location;
+    const ASTContext& context;
+    const Decl* decl;
+};
+inline Dump
+dump(loc loc, const ASTContext& context, const Decl* decl = nullptr) {
+    return {loc, context, decl};
+}
+raw_ostream& operator<<(raw_ostream&, Dump);
+
+// Print location in loc, falling back to address range of decl, falling
+// back to nothing.
+bool can_addr(loc loc, const Decl* decl = nullptr);
+struct Addr {
+    loc location;
+    const ASTContext& context;
+    const Decl* decl;
+};
+inline Addr
+addr(loc loc, const ASTContext& context, const Decl* decl = nullptr) {
+    return {loc, context, decl};
+}
+raw_ostream& operator<<(raw_ostream&, Addr);
+
+// Print diagnostic prefix "ADDR (DESCRIBE): " for loc, falling back to
+// "RANGE: " for decl, falling back to "".
+struct Prefix {
+    loc location;
+    const ASTContext& context;
+    const Decl* decl;
+};
+inline Prefix
+prefix(loc loc, const ASTContext& context, const Decl* decl = nullptr) {
+    return {loc, context, decl};
+}
+raw_ostream& operator<<(raw_ostream&, Prefix);
+
+// Print trace suffix "DESCRIBE at/in ADDR" for loc, falling back to "".
+inline bool
+can_trace(loc loc, const Decl* decl = nullptr) {
+    return loc.has_value();
+}
+struct Trace {
+    loc location;
+    const ASTContext& context;
+    const Decl* decl;
+};
+inline Trace
+trace(loc loc, const ASTContext& context, const Decl* decl = nullptr) {
+    return {loc, context, decl};
+}
+raw_ostream& operator<<(raw_ostream&, Trace);
+
+} // namespace loc
