include/Template.hpp
@@ -1,0 +1,33 @@
+/*
+ * Copyright (c) 2024 BedRock Systems, Inc.
+ * This software is distributed under the terms of the BedRock Open-Source License.
+ * See the LICENSE-BedRock file in the repository root for details.
+ */
+
+#pragma once
+#include <optional>
+
+namespace clang {
+class Decl;
+class NamedDecl;
+class TemplateDecl;
+class TemplateArgumentList;
+}
+
+/// Shallow view of template specialization
+struct SDecl {
+    const clang::TemplateDecl &temp;
+    const clang::TemplateArgumentList &args;
+
+    SDecl() = delete;
+    SDecl(const clang::TemplateDecl &t, const clang::TemplateArgumentList &a)
+        : temp{t}, args{a} {}
+};
+using SDeclO = std::optional<SDecl>;
+
+/**
+Attempt to decompose a declaration _directly_ into a template applied to
+arguments. This does not account for "untemplated" declarations in
+templated scopes.
+*/
+SDeclO recoverSpecialization(const clang::Decl &);
