src/Location.cpp
@@ -1,0 +1,259 @@
+/*
+ * Copyright (c) 2024 BedRock Systems, Inc.
+ * This software is distributed under the terms of the BedRock Open-Source License.
+ * See the LICENSE-BedRock file in the repository root for details.
+ */
+#include "Location.hpp"
+#include "Logging.hpp"
+#include <clang/Basic/Version.h>
+#include <clang/AST/ASTContext.h>
+#include <clang/AST/DeclCXX.h>
+#include <clang/AST/ExprCXX.h>
+
+using namespace clang;
+
+namespace structured {
+
+void
+locfree_warn(const Decl& decl, const ASTContext& context, StringRef msg) {
+    auto& os = logging::unsupported();
+    auto src = decl.getBeginLoc();
+    if (src.isValid()) {
+        src.print(os, context.getSourceManager());
+        os << ' ';
+    }
+    os << '(' << decl.getDeclKindName();
+    if (isa<NamedDecl>(decl)) {
+        os << ' ';
+        cast<NamedDecl>(decl).getNameForDiagnostic(
+            os, context.getPrintingPolicy(), true);
+    }
+    os << "): warning: " << msg << '\n';
+    decl.dump(logging::debug());
+}
+
+} // namespace structured
+
+namespace loc{
+
+template<> loc
+of<>(const DeclContext& c) {
+    return of(cast<Decl>(c));
+}
+
+template<> loc
+of<>(DeclContext& c) {
+    return of(cast<Decl>(c));
+}
+
+loc
+Loc::mk(const TypeLoc& t) {
+    if (t.getType().getTypePtrOrNull()) {
+        Loc::box<TypeLoc> box{&t};
+        Loc loc{box};
+        return {loc};
+    } else
+        return none;
+}
+
+loc
+Loc::mk(const TypeSourceInfo& t) {
+    if (t.getType().getTypePtrOrNull()) {
+        Loc::box<TypeSourceInfo> box{&t};
+        Loc loc{box};
+        return {loc};
+    } else
+        return none;
+}
+
+loc
+Loc::mk(const QualType& t) {
+    if (t.getTypePtrOrNull()) {
+        Loc::box<QualType> box{&t};
+        Loc loc{box};
+        return {loc};
+    } else
+        return none;
+}
+
+static constexpr SourceLocation invalid_loc;
+
+static SourceLocation
+pointOfInstantiation(const Decl& decl) {
+    if (auto ts = dyn_cast<ClassTemplateSpecializationDecl>(&decl))
+        return ts->getPointOfInstantiation();
+    if (auto fd = structured::recoverFunction(decl)) {
+        // NOTE: A FunctionDecl's POI can point uselessly into the
+        // template. The POIs FunctionDecl::getPointOfInstantiation and
+        // FunctionDecl::getTemplateSpecializationInfo;
+        // FunctionTemplateSpecialization::getPointOfInstantiation seem
+        // to always agree (unsurprisingly), even when they're "off".
+        return fd->getPointOfInstantiation();
+    }
+    if (auto ts = dyn_cast<VarTemplateSpecializationDecl>(&decl))
+        return ts->getPointOfInstantiation();
+    return invalid_loc;
+}
+
+static SourceLocation
+getDeclLoc(const Decl& decl) {
+    // Prefer point of instantiation
+    auto loc = pointOfInstantiation(decl);
+    return loc.isValid() ? loc : decl.getBeginLoc();
+}
+
+SourceLocation
+Loc::getLoc() const {
+    switch (kind) {
+    case Kind::Decl:	return getDeclLoc(*u.decl);
+    case Kind::Stmt:	return u.stmt->getBeginLoc();
+    case Kind::TypeLoc:	return u.typeloc->getBeginLoc();
+    case Kind::Tsi:	return u.tsi->getTypeLoc().getBeginLoc();
+    case Kind::QualType:
+    case Kind::Type:	return invalid_loc;
+    case Kind::Tal:	return u.tal->getSourceRange().getBegin();
+    }
+}
+
+raw_ostream&
+Loc::describe(raw_ostream& os, const ASTContext& context) const {
+    auto& policy = context.getPrintingPolicy();
+    auto qualtype = [&](QualType qt) -> auto& {
+        os << qt.getTypePtr()->getTypeClassName() << ' ';
+        qt.print(os, policy);
+        return os;
+    };
+    switch (kind) {
+    case Kind::Decl: {
+        auto decl = u.decl;
+        os << decl->getDeclKindName();
+        if (auto nd = dyn_cast<NamedDecl>(decl)) {
+            os << ' ';
+            structured::printNameForDiagnostics(os, *nd, context);
+        }
+        return os;
+    }
+    case Kind::Stmt:
+        return os << u.stmt->getStmtClassName();
+    case Kind::TypeLoc:
+        return qualtype(u.typeloc->getType());
+    case Kind::Tsi:
+        return qualtype(u.tsi->getType());
+    case Kind::QualType:
+        return qualtype(*u.qualtype);
+    case Kind::Type:
+        return qualtype(context.getQualifiedType(u.type, Qualifiers()));
+    case Kind::Tal:
+        u.tal->getArgument().print(policy, os, true);
+        return os;
+    }
+}
+
+template<typename T>
+void
+dump_ctx(raw_ostream& os, const T* t, const ASTContext& context) {
+    #if CLANG_VERSION_MAJOR >= 11
+        t->dump(os, context);
+    #else
+        t->dump(os);
+    #endif
+}
+
+raw_ostream&
+Loc::dump(raw_ostream& os, const ASTContext& context) const {
+    auto qualtype = [&](QualType qt) -> auto& {
+        dump_ctx(os, &qt, context);
+        return os;
+    };
+    switch (kind) {
+    case Kind::Decl:	u.decl->dump(os); return os;
+    case Kind::Stmt:	dump_ctx(os, u.stmt, context); return os;
+    case Kind::TypeLoc:	return qualtype(u.typeloc->getType());
+    case Kind::Tsi:	return qualtype(u.tsi->getType());
+    case Kind::QualType:	return qualtype(*u.qualtype);
+    case Kind::Type:	dump_ctx(os, u.type, context); return os;
+    case Kind::Tal:	u.tal->getArgument().dump(os); return os;
+    }
+}
+
+raw_ostream&
+operator<<(raw_ostream& os, Describe d) {
+    auto& [loc, context] = d;
+    return loc ? loc->describe(os, context) : os;
+}
+
+raw_ostream&
+operator<<(raw_ostream& os, Dump d) {
+    auto [loc, context, decl] = d;
+    if (loc)
+        loc->dump(os, context);
+    if (loc && decl)
+        os << "\tinside\n";
+    if (decl)
+        decl->dump(os);
+    if (loc || decl)
+        os << "\n"; // visually separate unrelated dumps
+    return os;
+}
+
+bool
+can_addr(loc loc, const Decl* decl) {
+    return (loc.has_value() && loc->getLoc().isValid()) || decl;
+}
+
+raw_ostream&
+operator<<(raw_ostream& os, Addr s) {
+    auto& [loc, context, decl] = s;
+    auto& SM = context.getSourceManager();
+    if (loc) {
+        auto src = loc->getLoc();
+        if (src.isValid()) {
+            src.print(os, SM);
+            return os;
+        }
+    }
+    if (decl)
+        decl->getSourceRange().print(os, SM);
+    return os;
+}
+
+raw_ostream&
+operator<<(raw_ostream& os, Prefix p) {
+    auto& [loc, context, decl] = p;
+    auto& SM = context.getSourceManager();
+    if (loc) {
+        auto src = loc->getLoc();
+        if (src.isValid()) {
+            src.print(os, SM);
+            os << " ";
+        } else if (decl) {
+            decl->getSourceRange().print(os, SM);
+            os << " ";
+        }
+        os << "(";
+        return loc->describe(os, context) << "): ";
+    } else if (decl) {
+        decl->getSourceRange().print(os, SM);
+        return os << ": ";
+    } else
+        return os;
+}
+
+raw_ostream&
+operator<<(raw_ostream& os, Trace t) {
+    auto& [loc, context, decl] = t;
+    if (loc) {
+        auto& SM = context.getSourceManager();
+        loc->describe(os, context);
+        auto src = loc->getLoc();
+        if (src.isValid()) {
+            os << " at ";
+            src.print(os, SM);
+        } else if (decl) {
+            os << " in ";
+            decl->getSourceRange().print(os, SM);
+        }
+    }
+    return os;
+}
+}
