src/Template.cpp
@@ -1,0 +1,35 @@
+/*
+ * Copyright (c) 2024 BedRock Systems, Inc.
+ * This software is distributed under the terms of the BedRock Open-Source License.
+ * See the LICENSE-BedRock file in the repository root for details.
+ */
+
+#include "Template.hpp"
+#include <clang/AST/DeclTemplate.h>
+
+using namespace clang;
+
+SDeclO
+recoverSpecialization(const Decl &decl) {
+    auto ret = [&](auto *temp, auto *args) -> SDeclO {
+        if (temp && args) {
+            SDecl sd{*temp, *args};
+            return {sd};
+        } else
+            return std::nullopt;
+    };
+    if (auto d = dyn_cast<ClassTemplateSpecializationDecl>(&decl)) {
+        auto* temp = d->getSpecializedTemplate();
+        auto& args = d->getTemplateArgs();
+        return ret(temp, &args);
+    } else if (auto d = dyn_cast<FunctionDecl>(&decl)) {
+        auto* temp = d->getPrimaryTemplate();
+        auto* args = d->getTemplateSpecializationArgs();
+        return ret(temp, args);
+    } else if (auto d = dyn_cast<VarTemplateSpecializationDecl>(&decl)) {
+        auto* temp = d->getSpecializedTemplate();
+        auto& args = d->getTemplateArgs();
+        return ret(temp, &args);
+    } else
+        return std::nullopt;
+}
