tests/cpp2v/name_test_id.t/run.t
@@ -1,0 +1,32 @@
+  $ . ../../setup-name-test.sh
+  $ name_test test.cpp
+  # cpp2v --name-test=test_17_name_test.v test.cpp -- -std=c++17
+  # scrub test_17_name_test.v
+  Require Import bedrock.auto.cpp.templates.mparser2.
+  
+  #[local] Open Scope bs_scope.
+  
+  Definition module_names : list Mname :=
+    (
+      (Nscoped
+        (Nglobal (Nid "ns")) (Nid "inhabit")) ::
+  
+      (Nglobal (Nid "c")) ::
+  
+      (Nglobal (Nid "s")) ::
+  
+      (Nglobal (Nid "u")) ::
+  
+      (Nglobal (Nid "e1")) ::
+  
+      (Nglobal (Nid "e2")) ::
+  
+      (Nglobal (Nid "t1")) ::
+  
+      (Nglobal (Nid "t2")) ::
+  
+      (Nglobal (Nid "v")) ::
+      nil).
+  
+  Definition template_names : list Mname :=
+    (nil).
